---
title: Abstract Algebra by Pinter, Chapter 16
author: Amir Taaki
header-includes: |
    - \usepackage{mathrsfs}
    - \usepackage{mathtools}
    - \usepackage{extpfeil}
abstract: Chapter 16 on Fundamental Homomorphism Theorem
---

# A. Examples of FHT

Use the FHT to prove that the two given groups are isomorphic. Then display their tables.

## Q1

$\mathbb{Z}_5$ and $\mathbb{Z}_{20} / \langle 5 \rangle$.

$$
\setcounter{MaxMatrixCols}{30}
f =
\begin{pmatrix}
0 & 1 & 2 & 3 & 4 & 5 & 6 & 7 & 8 & 9 & 10 & 11 & 12 & 13 & 14 & 15 & 16 & 17 & 18 & 19 \\
0 & 1 & 2 & 3 & 4 & 0 & 1 & 2 & 3 & 4 & 0 & 1 & 2 & 3 & 4 & 0 & 1 & 2 & 3 & 4 \\
\end{pmatrix}
$$

$$K = \{0, 5, 10, 15\} = \langle 5 \rangle$$

$$ f : \mathbb{Z}_{20} \underset{\langle 5 \rangle}{\relbar\joinrel\twoheadrightarrow} \mathbb{Z}_5 $$

$$ \mathbb{Z}_{5} \cong \mathbb{Z}_{20} / \langle 5 \rangle $$

## Q2

$\mathbb{Z}_3$ and $\mathbb{Z}_{6} / \langle 3 \rangle$.

$$
f =
\begin{pmatrix}
0 & 1 & 2 & 3 & 4 & 5 \\
0 & 1 & 2 & 0 & 1 & 2
\end{pmatrix}
$$

$$K = \{0, 3\} = \langle 3 \rangle$$

$$ f : \mathbb{Z}_{6} \underset{\langle 3 \rangle}{\relbar\joinrel\twoheadrightarrow} \mathbb{Z}_3 $$

$$ \mathbb{Z}_{3} \cong \mathbb{Z}_{6} / \langle 3 \rangle $$

## Q3

$\mathbb{Z}_2$ and $S_3 / \{ \epsilon, \beta, \delta \}$.

$$
f =
\begin{pmatrix}
\epsilon & \alpha & \beta & \gamma & \delta & \kappa \\
0        & 1      & 0     & 1      & 0      & 1      \\
\end{pmatrix}
$$

$$K = \{ \epsilon, \beta, \delta \} $$

$$ f : S_3 \underset{\{ \epsilon, \beta, \delta \}}{\relbar\joinrel\twoheadrightarrow} \mathbb{Z}_2 $$

$$ \mathbb{Z}_{2} \cong S_3 / \{ \epsilon, \beta, \delta \} $$

## Q4

From Chapter 3, part C (at the end):

$$ P_D = \{ A : A \subseteq D \} $$

If $A$ and $B$ are any two sets, their symmetric difference is the set $A + B$ defined as follows:

$$ A + B = (A - B) \cup (B - A) $$

$A - B$ represents the set obtained by removing from $A$ all the elements which are in $B$.

$$ P_3 = \{ \varnothing, \{a\}, \{b\}, \{c\}, \{a, b\}, \{a, c\}, \{b, c\}, \{a, b, c\} \} $$

Consider the function $f(C) = C \cap \{a, b\}$

$$ P_2 = \{ \varnothing, \{a\}, \{b\}, \{a, b\} \} $$

The kernel is $\{ \varnothing, \{ c \} \}$

Using the kernel we create the quotient cosets:

\begin{align*}
K &= \{ \varnothing, \{ c \} \} \\
&= K + \{ c \} \\
K + \{ a \} &= \{ \{ a \}, \{ a, c \} \} \\
&= K + \{ a, c \} \\
K + \{ b \} &= \{ \{ b \}, \{ b, c \} \} \\
&= K + \{ b, c \} \\
K + \{ a, b \} &= \{ \{ a, b \}, \{ a, b, c \} \} \\
&= K + \{ a, b, c \} \\
\end{align*}

Applying the function to the cosets, we get:

\begin{align*}
f(K) &= \{ \varnothing \} \\
f(K \cap \{ a \}) &= \{ \{ a \} \} \\
f(K \cap \{ b \}) &= \{ \{ b \} \} \\
f(K \cap \{ a, b \}) &= \{ \{ a, b \} \} \\
\end{align*}

Thus,

$$ f : P_3 \underset{\{ \varnothing, \{ c \} \}}{\relbar\joinrel\twoheadrightarrow} P_2 $$

$$ P_2 \cong P_3 / \{ \varnothing, \{ c \} \} $$

## Q5

$\mathbb{Z}_3$ and $(\mathbb{Z}_3 \times \mathbb{Z}_3) / K$ where $K = \{ (0, 0), (1, 1), (2, 2) \}$

Consider $f: \mathbb{Z}_3 \times \mathbb{Z}_3 \rightarrow \mathbb{Z}_3$ by:

$$ f(a, b) = a - b $$

$$ \mathbb{Z}_3 \times \mathbb{Z}_3 = \{ (0, 0), (0, 1), (0, 2), (1, 0), (1, 1), (1, 2), (2, 0), (2, 1), (2, 2) \} $$

\begin{alignat*}{2}
\bar{(0, 0)} &= K + (0, 0) &= K + (1, 1) &= K + (2, 2) \\
\bar{(0, 1)} &= K + (0, 1) &= K + (1, 2) &= K + (2, 0) \\
\bar{(0, 2)} &= K + (0, 2) &= K + (1, 0) &= K + (2, 1) \\
\end{alignat*}

Applying the function to any element $k$ from the cosets we get:

\begin{alignat*}{2}
f(0, 0) &= f(1, 1) &= f(2, 2) = 0 \\
f(0, 1) &= f(1, 2) &= f(2, 0) = 2 \\
f(0, 2) &= f(1, 0) &= f(2, 1) = 1
\end{alignat*}

Thus,

$$ f : \mathbb{Z}_3 \times \mathbb{Z}_3 \underset{K}{\relbar\joinrel\twoheadrightarrow} \mathbb{Z}_3 $$

$$ \mathbb{Z}_3 \cong \mathbb{Z}_3 \times \mathbb{Z}_3 / \{ (0, 0), (1, 1), (2, 2) \} $$

# B. Example of the FHT Applied to $F(\mathbb{R})$

## Q1

Let $\alpha : F(\mathbb{R}) \rightarrow \mathbb{R}$ be:

$$ \alpha (f) = f(1) $$

Let $\beta : F(\mathbb{R}) \rightarrow \mathbb{R}$ be:

$$ \beta (f) = f(2) $$

Prove $\alpha$ and $\beta$ are homomorphisms from $F(\mathbb{R})$ onto $\mathbb{R}$.

Let $g, h \in F(\mathbb{R})$, then:

\begin{align*}
f(g + h) &= (g + h)(1) \\
         &= g(1) + h(1)
\end{align*}

Likewise for $\beta$

The functions are onto because the range of each function are $f(1)$ and $f(2)$ respectively.

## Q2

$$ J = \{ f : f(1) = 0, \forall f \in F(\mathbb{R}) \} $$
$$ K = \{ f : f(2) = 0, \forall f \in F(\mathbb{R}) \} $$

The cosets of $F(\mathbb{R})$ for $\alpha$ are:

$$ J + g, \forall g \in F(\mathbb{R}) $$

And for $\beta$:

$$ K + g, \forall g \in F(\mathbb{R}) $$

## Q3

For any arbitrary $g, h \in F(\mathbb{R})$ and $k_1, k_2 \in J$,

\begin{align*}
f((k_1 + g) + (k_2 + h)) &= (k_1 + g + k_2 + h)(1) \\
                         &= f(k_1 + g) + f(k_2 + h)
\end{align*}

Thus $J + g$ and $K + g$ are valid quotient groups.

$J$ and $K$ have the same cardinality under $F(\mathbb{R})$ and so:

$$ F(\mathbb{R}) / J \cong F(\mathbb{R}) / K $$

# C. Example of FHT with Abelian Groups

## Q1

Let $a, b \in G$

$$ f(ab) = (ab)^2 $$

But $G$ is abelian, so:

\begin{align*}
(ab)^2 &= a^2 b^2 \\
       &= f(a) f(b)
\end{align*}

And $H = \{ x^2 : x \in G \}$

So $f$ is a homomorphism of $G$ onto $H$

## Q2

$ker(f)$ is defined as:

\begin{align*}
K &= \{ x \in G : f(x) = e \} \\
  &= \{ x \in G : x^2 = e \}
\end{align*}

## Q3

$f: G \rightarrow H$ is a homomorphism of $G$ onto $H$, with a kernel K,
$f : G \underset{K}{\relbar\joinrel\twoheadrightarrow} H$
So therefore,

$$ H \cong G/K $$

# D. Group of Inner Automorphisms

See also the videos by Elliot724 on YouTube about automorphisms.

## Q1

For $Aut(G) \subseteq S_G$, prove $Aut(G) \leq S_G$.

We must prove that $Aut(G)$ obeys the group axioms.

Definition of $Aut(G)$:

$$ Aut(G) = \{ f \in S_G : f(g_1 g_2) = f(g_1) f(g_2), \forall g_1, g_2 \in G \} $$

Therefore for any $f_1, f_2 \in Aut(G)$, it is true that:

$$\forall g_1, g_2 \in G, f_1(f_2(g_1 g_2)) = f_1(f_2(g_1)) f_1(f_2(g_2))$$

Set obeys **closure** property.

Secondly there is an **identity** element $f_e \in S_G$ such that $f_e: g \rightarrow g, \forall g \in G$. Thus $f_e \in Aut(G)$.

Lastly $\forall f \in Aut(G), \forall g_1, g_2 \in G$, that there exists:

\begin{align*}
f(\bar{g_1}) &= g_1 \\
f(\bar{g_2}) &= g_2 \\
\end{align*}

Because $f$ is bijective, in particular from the surjective property, we can compose elements in the domain.

\begin{align*}
f(\bar{g_1} \bar{g_2}) &= f(\bar{g_1}) f(\bar{g_2}) \\
                       &= g_1 g_2
\end{align*}

Now because know that:

$$ f^{-1}(g_1 g_2) = f^{-1}(g_1) f^{-1}(g_2) $$

Substituting in the values of $g_1$ and $g_2$, we get:

\begin{align*}
f^{-1}(f(\bar{g_1} \bar{g_2})) &= f^{-1}(f(\bar{g_1})) f^{-1}(f(\bar{g_2})) \\
           \bar{g_1} \bar{g_2} &= \bar{g_1} \bar{g_2}
\end{align*}

Thus group has an **inverse**.

$$ Aut(G) \leq S_G $$

## Q2

$\phi_a$ denotes an inner automorphism of $G$:

$$ \text{for every } x \in G \qquad \phi_a(x) = axa^{-1} $$

Prove every inner automorphism is an automorphism of $G$.

$$ \phi_a(x) = axa^{-1} $$

Show homomorphic property:

$$ \phi_a(xy) = axya^{-1} $$

But $e = a^{-1} a$, so:
$$ \phi_a(xy) = ax(a^{-1} a)ya^{-1} = \phi_a(x) \phi_a(y) $$

So $\phi_a$ is homomorphic.

Also $\phi_e(x) = x \quad \forall x \in G$

## Q3

Likewise from above:

$$ \phi_a \cdot \phi_b = \phi_{ab} $$

Because $a(bxb^{-1})a^{-1} = (ab)x(ab)^{-1}$

For the inverse, we note that:

\begin{align*}
\phi_a(x) \phi_b(x) &= \phi_e(x) = x \\
                    &= (ab) x (ab)^{-1}
\end{align*}

It therefore follows that the inverse automorphism of $\phi_a$ is:

$$ (\phi_a)^{-1} = \phi_{a^{-1}} $$

## Q4

$I(G) = \{ \phi_a : a \in G \}$. Prove $I(G) \leq Aut(G)$.

**Closure**: for any $\phi_a, \phi_b \in I(G)$, then $\phi_a \cdot \phi_b \in I(G)$ because $\phi_a \cdot \phi_b = \phi_{ab}$

**Identity**: $\phi_e$ is the identity because $eae^{-1} = a$, so $\phi_e \in I(G)$.

**Inverses**: $\forall \phi_a \in I(G)$, there is an $\phi_{a^{-1}} \in I(G)$ because $\phi_a \cdot \phi_{a^{-1}} = \phi_{a a^{-1}} = \phi_e$, thus $\phi_{a^{-1}} = (\phi_a)^{-1}$

## Q5

$$ C = \{ a \in G : ax = xa \text{ for every } x \in G \} $$

Let $a \in C$. Then for every $x \in G$:

$$ ax = xa \text{ or } axa^{-1} = x $$

## Q6

Let $h: G \rightarrow I(G)$ be a function defined by $h(a) = \phi$. Prove that $h$ is a homomorphism from $G$ *onto* $I(G)$ and that $C$ is its kernel.

We can see that $h(ab) = \phi_{ab} = \phi_a \cdot \phi_b = h(a) h(b)$. Lastly the function is surjective (onto) because for every $\phi$, there is a corresponding $a \in G$ (possibly multiple if for example the group is abelian), so the mapping is well defined.

The kernel is defined by:

$$ K = \{ x \in G : f(x) = e \} $$

In our case this is:

$$ K = \{ a \in G : h(a) = \phi_e \} $$

The center is defined as:

$$ C = \{ a \in G : axa^{-1} = x \text{ for every } x \in G \} $$

Which is also the same as writing:

$$ K = \{ a \in G : h(a) = \phi_e \} $$

## Q7

Lastly using the FHT, we note that:

$$ h : G \underset{C}{\relbar\joinrel\twoheadrightarrow} I(G) $$

$$ I(G) \cong G / C $$

# E. FHT Applied to Direct Products of Groups

## Q1

Let $G$ and $H$ be groups.

Suppose $J \trianglelefteq G$ and $K \trianglelefteq H$

$$f(x, y) = (Jx, Ky)$$

Assuming $x \in G$ and $y \in H$, then $Jx$ and $Ky$ form the cosets for $G$ and $H$.

That is for every value from $G$ and $H$ maps onto $(G / J) \times (H / K)$ because:

$$x \in J\bar{x} \iff Jx = J\bar{x}$$
$$y \in K\bar{y} \iff Ky = K\bar{y}$$

$$f: G \times H \rightarrow (G/J) \times (H/K)$$

## Q2

$$ker f = \{ (x, y) \in G \times H : f(x, y) = (J, K) \} = J \times K$$

## Q3

$$ f : G \times H \underset{J \times K}{\relbar\joinrel\twoheadrightarrow} (G/J) \times (H/K) $$

$$ (G\times H)/(J \times K) \cong (G/J) \times (H/K) $$

# F. First Isomorphism Theorem

## Q1

$K \leq G, H \trianglelefteq G$

Both $H$ and $K$ are closed subgroups, so an element in both must by definition remain within $H \cap K$.

Let $h \in H \cap K$, then $\forall x \in G, xax^{-1} \in H$. This also applies to $K$. Therefore $H \cap K$ is a normal subgroup of $K$.

## Q2

$HK = \{ xy : x \in H \text{ and } y \in K \}$. Prove $HK$ is a subgroup of $G$.

Let $a, b \in HK$, then $ab = (h_1 k_1)(h_2 k_2) = h_1 (k_1 h_2 k_1^{-1}) k_1 k_2$ which is another element in $HK$.

## Q3

$H$ is a normal subgroup of $HK$.

Since $HK$ is a subgroup of $G$ then every element of $H$ conjugated with elements from $HK$ also lay within $H$.

$H \trianglelefteq HK$

## Q4

Let $x \in HK$ then $x = hk$ for some $h \in H, k \in K$. Form the coset $Hx = H(hk) = Hk$.

Thus $HK/H$ may be written as $Hk$ for some $k \in K$.

## Q5

Prove $f(k) = Hk$ is a homomorphism $f: K \rightarrow HK/H$, and its kernel is $H \cap K$

Since $Hk_1 = Hk_2$ for $k_1, k_2$ in the same coset, then any member of the quotient group $HK/H$ is equal to $H$ multiplied by a representative from that member.

To find the kernel, we need every $x \in K$ such that $f(x) = H$, the identity coset. That is $x \in H$. But since we are mapping from $K$, then $x \in K$ and $x \in H$. In other words, $ker f = H \cap K$.

## Q6

$$ f : K \underset{H \cap K}{\relbar\joinrel\twoheadrightarrow} HK/H $$

$$ K/(H \cap K) \cong HK/H $$

