---
title: Abstract Algebra by Pinter, Chapter 17
author: Amir Taaki
header-includes: |
    - \usepackage{mathrsfs}
    - \usepackage{mathtools}
    - \usepackage{extpfeil}
    - \DeclareMathOperator\cis{cis}
    - \DeclareMathOperator\ker{ker}
    - \DeclareMathOperator\ord{ord}
    - \DeclareMathOperator\gcd{gcd}
    - \DeclareMathOperator\lcm{lcm}
abstract: Chapter 17 on Rings
---

# A. Examples of Rings

Prove that the following are commutative rings with unity.

Indicate the zero element, the unity and the negative for an $a$.

Ring axioms:

1. $a \oplus b = b \oplus a$
2. $(a \otimes b) \otimes c = a \otimes (b \otimes c)$
3. $a \otimes (b \oplus c) = (a \otimes b) \oplus (a \otimes c)$

Commutative:

1. $a \otimes b = b \otimes a$

With unity:

1. $\exists 1' \in A : a \otimes 1' = a$

## Q1

$$a \oplus b = a + b - 1 \qquad a \otimes b = ab - (a + b) + 2$$

Axiom 1 is self evident.

Using sage, we prove axioms 2 and 3.

```python
sage: a = var('a')
sage: b = var('b')
sage: c = var('c')
sage: ab = a*b - (a + b) + 2
sage: ab_c = ab*c - (ab + c) + 2
sage: bc = b*c - (b + c) + 2
sage: a_bc = a*bc - (a + bc) + 2
sage: ab_c.full_simplify()
-(a - 1)*b + ((a - 1)*b - a + 1)*c + a
sage: a_bc.full_simplify()
-(a - 1)*b + ((a - 1)*b - a + 1)*c + a
```

```python
sage: def mul(a, b):
....:     return a*b - (a + b) + 2
....: 
sage: def add(a, b):
....:     return a + b - 1
....: 
sage: mul(a, add(b, c)).full_simplify()
(a - 1)*b + (a - 1)*c - 2*a + 3
sage: add(mul(a, b), mul(a, c)).full_simplify()
(a - 1)*b + (a - 1)*c - 2*a + 3
```

To calculate zero and unity:

$$a \oplus 0' = a$$
$$a + b - 1 = a$$
$$b = 1 = 0'$$

$$a \otimes 1' = a$$
$$ab - (a + b) + 2 = a$$
$$b = 2 = 1'$$

Lastly for the negative:

$$a \oplus b = 0'$$
$$a + b - 1 = 1$$
$$b = -a$$

## Q2

$$a \oplus b = a + b + 1 \qquad a \otimes b = ab + a + b$$

```python
sage: def add(a, b):
....:     return a + b + 1
....: 
sage: def mul(a, b):
....:     return a*b + a + b
```

Axiom 1: $a \oplus b = b \oplus a$

*Self-evident*

Axiom 2: $(a \otimes b) \otimes c = a \otimes (b \otimes c)$

```python
sage: bool(mul(mul(a, b), c) == mul(a, mul(b, c)))
True
```

Axiom 3: $a \otimes (b \oplus c) = (a \otimes b) \oplus (a \otimes c)$

```python
sage: bool(mul(a, add(b, c)) == add(mul(a, b), mul(a, c)))
True
```

Commutative: $a \otimes b = b \otimes a$

*Self-evident*

Zero:

```python
sage: solve(add(a, b) - a, b)
[b == -1]
sage: add(a, -1)
a
```

Unity:

```python
sage: solve(mul(a, b) - a, b)
[b == 0]
sage: mul(a, 0)
a
```

Negative $a$:

```python
sage: solve(add(a, b) + 1, b)
[b == -a - 2]
sage: add(a, -a -2)
-1
```

## Q3

$$(a, b) \oplus (c, d) = (a + c, b + d)$$
$$(a, b) \otimes (c, d) = (ac - bd, ad + bc)$$

```python
sage: c = var('c')
sage: d = var('d')
sage: e = var('e')
sage: f = var('f')
sage: def add(ab, cd):
....:     a, b = ab
....:     c, d = cd
....:     return (a + c, b + d)
....: 
sage: def mul(ab, cd):
....:     a, b = ab
....:     c, d = cd
....:     return (a*c - b*d, a*d + b*c)
....: 

```

Axiom 1: $a \oplus b = b \oplus a$

```python
sage: bool(add((a, b), (c, d)) == add((c, d), (a, b)))
True
```

Axiom 2: $(a \otimes b) \otimes c = a \otimes (b \otimes c)$

```python
sage: bool(mul(mul((a, b), (c, d)), (e, f)) == mul((a, b), mul((c, d), (e, f))))
True
```

Axiom 3: $a \otimes (b \oplus c) = (a \otimes b) \oplus (a \otimes c)$

```python
sage: bool(mul((a, b), add((c, d), (e, f))) == add(mul((a, b), (c, d)), mul((a, b), (e, f))))
True
```

Commutative: $a \otimes b = b \otimes a$

*Self-evident*

Zero:

```python
sage: ab_plus_cd = add((a, b), (c, d))
sage: solve(ab_plus_cd[0] - a, c)
[c == 0]
sage: solve(ab_plus_cd[1] - b, d)
[d == 0]
sage: add((a, b), (0, 0))
(a, b)
```

Unity:

```python
sage: ab_mul_cd = mul((a, b), (c, d))
sage: solve([ab_mul_cd[0] - a, ab_mul_cd[1] - b], c, d)
[[c == 1, d == 0]]
sage: mul((a, b), (1, 0))
(a, b)
```

Negative $a$:

Since $0' = (0, 0)$ then the negative for $(a, b)$ is simply $(-a, -b)$.

## Q4

$$A = \{ x + y\sqrt{2} : x, y \in \mathbb{Z} \}$$

Since normal algebraic operations are defined on A, then 1, 2 and 3 pass. It is also commutative.

Zero: 0

Unity: 1

Negative: $-x -y\sqrt{2}$

## Q5

Prove the ring in part 1 is an integral domain.

We show that it has the cancellation property.

Assume $a \otimes b = a \otimes c$.

$$ab - (a + b) + 2 = ac - (a + c) + 2$$
$$ab - b = ac - c$$

Therefore $b = c$, and the ring has the cancellation property.

## Q6

Prove the ring in part 2 is a field.

A field is a commutative ring with unity in which every nonzero element is invertible.

$$0' = -1$$
$$1' = 0$$

Thus

$$a \otimes b = 1'$$
$$ab + a + b = 0$$

We solve for b as follows

```python
sage: def mul(a, b):
....:         return a*b + a + b
....: 
sage: solve(mul(a, b), b)
[b == -a/(a + 1)]
```

(Excluding the $0'$ element which is equal to $-1$)

## Q7

Find the inverse for the ring in part 3.

```python
sage: def mul(ab, cd):
....:     a, b = ab
....:     c, d = cd
....:     return (a*c - b*d, a*d + b*c)
....: 
sage: ab_mul_cd = mul((a, b), (c, d))
sage: solve([ab_mul_cd[0] - 1, ab_mul_cd[1]], c, d)
[[c == a/(a^2 + b^2), d == -b/(a^2 + b^2)]]
```

# B. Ring of Real Functions

## Q1

Let $a, b \in \mathcal{F}(\mathbb{R})$

Ring axioms:

1. $ab = ba$
2. $(ab)c = a(bc)$
3. $a(b + c) = ab + ac$

Commutative:

1. ab = ba

Zero: $f(x) = 0$

Unity: $f(x) = 1$

Negative: $-f(x)$

## Q2

Divisors of zero, are any two functions which when $f(x) \neq 0$ then $g(x) = 0$ but in general $f(x) \neq 0$ and $g(x) \neq 0$.

See [more here](https://math.stackexchange.com/questions/827448/zero-divisors-in-ring-of-real-valued-functions)

## Q3

Any functions which are one to one and have an inverse. That is $f(x) = x^3$ but not $f(x) = x^2$.

## Q4

A field must have every element invertible. So the ring is not a field.

Ring has divisors of zero, so it does not have the cancellation property $\implies$ ring is not an integral domain.

# C. Ring of $2 \times 2$ Matrices

## Q1

```python
sage: a = var('a')
sage: b = var('b')
sage: c = var('c')
sage: d = var('d')
sage: r = var('r')
sage: s = var('s')
sage: t = var('t')
sage: u = var('u')
sage: w = var('w')
sage: x = var('x')
sage: y = var('y')
sage: z = var('z')
sage: 
sage: def add(abcd, rstu):
....:     a, b, c, d = abcd
....:     r, s, t, u = rstu
....:     return (a + r, b + s, c + t, d + u)
....: 
sage: def mul(abcd, rstu):
....:     a, b, c, d = abcd
....:     r, s, t, u = rstu
....:     return (a*r + b*t, a*s + b*u, c*r + d*t, c*s + d*u)
```

Axiom 1: 

*Self evident.*

Axiom 2:

```python
sage: bool(mul((a,b,c,d), mul((r,s,t,u), (w,x,y,z))) == mul(mul((a,b,c,d), (r,s,t,u)), (w,x,y,z
....: )))
True
```

Axiom 3:

```python
sage: bool(mul((a,b,c,d), add((r,s,t,u), (w,x,y,z))) == add(mul((a,b,c,d), (r,s,t,u)), mul((a,b
....: ,c,d), (w,x,y,z))))
True
```

## Q2

```python
sage: bool(mul((a,b,c,d), (r,s,t,u)) == mul((r,s,t,u), (a,b,c,d)))
False
```

Unity: $(a,b,c,d)(r,s,t,u) = (a, b, c,d)$

```python
sage: solve([x_mul_y[0] - a, x_mul_y[1] - b, x_mul_y[2] - c, x_mul_y[3] - d], r,s,t,u)
[[r == 1, s == 0, t == 0, u == 1]]
```

$$
I =
\begin{pmatrix}
1 & 0\\
0 & 1
\end{pmatrix}
$$

## Q3

Matrices don't have the cancellation property.

For example $ar_1 + bt_1 = ar_2 + bt_2$ does not imply that $r_1 = r_2$ and $t_1 = t_2$.

Thus is not an integral domain.

Not all matrices are invertible, for example when $det(A) = 0$. See more info [here](https://en.wikipedia.org/wiki/Cancellation_property#Non-cancellative_algebraic_structures). Hence they $\mathcal{M}_2(\mathbb{R})$ is not a field either.

# D. Rings of Subsets of a Set

$$A + B = (A - B) \cup (B - A)$$
$$AB = A \cap B$$

## Q1

Ring axioms:

1. \begin{align*}
A + B &= (A - B) \cup (B - A) \\
      &= B + A
\end{align*}
2. $$(AB)C = (A \cap B)\cap C = A \cap (B \cap C) = A(BC)$$
3. \begin{align*}
A(B+C) &= A\cap [(B - C) \cup (C -B)] \\
       &= [A \cap (B - C)] \cup [A \cap (C - B) ] \\
       &= (AB - AC) \cup (AC - AB) \\
AB + AC &= (AB - AC) \cup (AC - AB)
\end{align*}

Commutativity:

$$AB = A \cap B = BA$$

Unity:

$$AB = A \implies B = D$$

Zero:

$$A + B = A \implies B = \varnothing$$

## Q2

All elements of $P_D$ with non-overlapping regions are divisors of zero.

$$X \in P_D, X^2 = \varnothing$$

## Q3

$$1' = D$$
$$AB = D \implies A \cap B = D$$
Thus $A = D$ and $B = D$

## Q4

There exist non-zero non-invertible elements in $P_D$, hence it is *not* a field.

$AB = AC$ does not imply $B = C$, hence cancellation property does not hold, and $P_D$ is not an integral domain.

## Q5

\begin{align*}
e = \varnothing \\
a = \{a\} \\
b = \{b\} \\
c = \{c\} \\
ab = \{a, b\} \\
ac = \{a, c\} \\
bc = \{b, c\} \\
abc = \{a, b, c\}
\end{align*}

\begin{tabular}{c | c c c c c c c c c}
    $\oplus$ & e & a & b & c & ab & ac & bc & abc \\
    \cline{1-9}
    e & e   & a   & b   & c   & ab  & ac  & bc  & abc \\
    a & a   & e   & ab  & ac  & b   & c   & abc & bc  \\
    b & b   & ab  & e   & bc  & a   & abc & c   & ac  \\
    c & c   & ac  & bc  & e   & abc & a   & b   & ab  \\
   ab & ab  & b   & a   & abc & e   & bc  & ac  & c   \\
   ac & ac  & c   & abc & a   & bc  & e   & ab  & b   \\
   bc & bc  & abc & c   & b   & ac  & ab  & e   & a   \\
  abc & abc & bc  & ac  & ab  & c   & b   & a   & e   \\
\end{tabular}

\begin{tabular}{c | c c c c c c c c c}
    $\otimes$ & e & a & b & c & ab & ac & bc & abc \\
    \cline{1-9}
    e & e   & a   & b   & c   & ab  & ac  & bc  & abc \\
    a & a   & a   & ab  & ac  & ab  & ac  & abc & abc \\
    b & b   & ab  & b   & bc  & ab  & abc & bc  & abc \\
    c & c   & ac  & bc  & e   & abc & a   & b   & abc \\
   ab & ab  & ab  & ab  & abc & ab  & abc & abc & abc \\
   ac & ac  & ac  & abc & ac  & abc & ac  & abc & abc \\
   bc & bc  & abc & bc  & bc  & abc & abc & bc  & abc \\
  abc & abc & abc & abc & abc & abc & abc & abc & abc \\
\end{tabular}

# E. Ring of Quaternions

## Q1

Unity:

```python
sage: a = var('a')
sage: b = var('b')
sage: c = var('c')
sage: d = var('d')
sage: matrix([[a + b*I, c + d*I], [-c + d*I, a - b*I]])
[ a + I*b  c + I*d]
[-c + I*d  a - I*b]
sage: alpha = matrix([[a + b*I, c + d*I], [-c + d*I, a - b*I]])
sage: matrix([[1, 0], [0, 1]]) * alpha
[ a + I*b  c + I*d]
[-c + I*d  a - I*b]
```

Distributive law:

```python
sage: bb = var('e f g h')
sage: cc = var('i j k l')
sage: def make_matrix(xx):
....:     return matrix([[xx[0] + I*xx[1], xx[2] + xx[3]*I], [-xx[2] + xx[3]*I, xx[0] - xx[1]*I]])
....: 
sage: bool(alpha*(make_matrix(bb) + make_matrix(cc)) == (alpha*make_matrix(bb) + alpha*make_matrix(cc)))
True
```

Non-commutative:

```python
sage: bool(alpha*make_matrix(bb) == make_matrix(bb)*alpha)
False
```

## Q2

$$
\mathbf{1} = 
\begin{pmatrix}
1 & 0\\
0 & 1
\end{pmatrix}
$$

$$
\mathbf{i} = 
\begin{pmatrix}
i & 0\\
0 & -i
\end{pmatrix}
$$

$$
\mathbf{j} = 
\begin{pmatrix}
0 & 1\\
-1 & 0
\end{pmatrix}
$$

$$
\mathbf{k} = 
\begin{pmatrix}
0 & i\\
i & 0
\end{pmatrix}
$$

\begin{align*}
\alpha &= a \mathbf{1} + b \mathbf{i} + c \mathbf{j} + d \mathbf{k} \\
       &=    
\begin{pmatrix}
a + bi & c + di\\
-c + di & a - bi
\end{pmatrix}
\end{align*}

## Q3

For the formula $\mathbf{i}^2 = \mathbf{j}^2 = \mathbf{k}^2 = -\mathbf{1}$

```python
sage: ii = matrix([[I, 0], [0, -I]])
sage: ii*ii
[-1  0]
[ 0 -1]
sage: -ii*ii
[1 0]
[0 1]
sage: jj = matrix([[0, 1], [-1, 0]])
sage: jj*jj
[-1  0]
[ 0 -1]
sage: kk = matrix([[0, I], [I, 0]])
sage: kk*kk
[-1  0]
[ 0 -1]
sage: bool(ii**2 == jj**2)
True
sage: bool(ii**2 == kk**2)
True
```

$\mathbf{ij} = -\mathbf{ji} = \mathbf{k}$

```python
sage: bool(ii*jj == -jj*ii)
True
sage: bool(ii*jj == kk)
True
```

$\mathbf{jk} = -\mathbf{kj} = \mathbf{i}$

```python
sage: bool(jj*kk == -kk*jj)
True
sage: bool(jj*kk == ii)
True
```

$\mathbf{ki} = -\mathbf{ik} = \mathbf{j}$

```python
sage: bool(kk*ii == -ii*kk)
True
sage: bool(kk*ii == jj)
True
```

## Q4

$$\bar{\alpha} =
\begin{pmatrix}
a - bi & -c - di\\
c - di & a + bi
\end{pmatrix}
$$

$$||\alpha|| = a^2 + b^2 + c^2 + d^2 = t$$

Show that

$$
\bar{\alpha}\alpha = \alpha\bar{\alpha} =
\begin{pmatrix}
t & 0\\
0 & t
\end{pmatrix}
$$

```python
sage: alpha
[ a + I*b  c + I*d]
[-c + I*d  a - I*b]
sage: alpha_bar = matrix([[a - b*I, -c - d*I], [c - d*I, a + b*I]])
sage: bool(alpha_bar*alpha == alpha*alpha_bar)
True
sage: alpha_bar*alpha
[(a + I*b)*(a - I*b) + (c + I*d)*(c - I*d)                                         0]
[                                        0 (a + I*b)*(a - I*b) + (c + I*d)*(c - I*d)]
```

Note that $(a + ib)(a - ib) = a^2 + b^2$ and the same for $c$ and $d$.

Earlier we found the identity is

$$
\mathbf{1} =
\begin{pmatrix}
1 & 0\\
0 & 1
\end{pmatrix}
$$

Thus the multiplicative inverse (both on the left and right) such that $\alpha\beta = \beta\alpha = \mathbf{1}$ is given by $(1/t)\bar{\alpha}$.

## Q5

From part 4 we show there is a multiplicative inverse. Thus by the definition, $\mathcal{L}$ is a skew field.
